Updated Curve25519_Operations with latest proof

proof/crypto_scalarmult/curve25519/amd64/common/Curve25519_Operations.ec
@@ -1,47 +1,34 @@
-require import Bool List Int IntExtra IntDiv CoreMap Real Zp.
+require import Bool List Int IntDiv CoreMap Real Ring StdOrder Zp_25519 Zp_limbs Eclib.
 from Jasmin require import JModel.
 require import Curve25519_Spec.
-import Zp ZModpRing.
+import Zp StdOrder.IntOrder Ring.IntID Array4 EClib.
+
+(* sets last bit to 0 *) 
+op last_bit_to_zero64 (x: Rep4) : Rep4 = let x = x.[3 <- x.[3].[63 <- false]] in x.
 
 (* returns the first 2 elements of the input triple *)
-op select_tuple_12 (t : ('a * 'a) * ('a * 'a) * 'c) = (t.`1, t.`2).
+op select_double_from_triple (t : ('a * 'a) * ('a * 'a) * 'c) : ('a * 'a) * ('a * 'a) = (t.`1, t.`2).
 
 (* if the third element is true then the first 2 elements are swapped *)
 (*  - this op returns the first 2 elements in the correct order       *)
-op reconstruct_tuple (t : ('a * 'a) * ('a * 'a) * bool) =
+op reconstruct_triple (t : ('a * 'a) * ('a * 'a) * bool) : ('a * 'a) * ('a * 'a)  =
   if t.`3
-  then swap_tuple (select_tuple_12 t)
-  else select_tuple_12 t.
+  then spec_swap_tuple (select_double_from_triple t)
+  else select_double_from_triple t.
 
-lemma eq_reconstruct_select_tuple (t : (('a * 'a) * ('a * 'a) * bool)) :
+(* given that t.`3 is false, we can convert from a "list" with two elems
+   to a ""list"" with three elements, whereby the last element is false *)
+lemma eq_reconstruct_select_triple (t : (('a * 'a) * ('a * 'a) * bool)) :
   t.`3 = false =>
-  select_tuple_12 t = reconstruct_tuple t.
+  select_double_from_triple t = reconstruct_triple t.
 proof.
-  rewrite /reconstruct_tuple /select_tuple_12.
+  rewrite /reconstruct_triple /select_double_from_triple.
   by move => ? /#.
 qed.
 
-(* similar to foldl_in_eq -- the proof is basically the same -- defined in JMemory *)
-(* - foldl_in_eq states that any 2 foldl's are the same if the functions are equiv *)
-(* - we will need to prove that + that the state a2 have a relational invariant r  *)
-lemma foldl_in_eq_r (f1 : 'a1 -> 'b -> 'a1)
-                    (f2 : 'a2 -> 'b -> 'a2)
-                    (s  : 'b list)
-                    (a2 : 'a2)
-                    (r  : 'a2 -> 'a1) :
-(forall a2 b, b \in s => f1 (r a2) b = r (f2 a2 b)) => foldl f1 (r a2) s = r (foldl f2 a2 s).
-proof.
-  move: s a2. elim.
-  by move => a2.
-  move => x l hrec a2 /= hin. rewrite hin.
-  by left.
-  rewrite hrec //; move => ? ? h; rewrite hin.
-  by right.
-  by trivial.
-qed.
 
 (** step1: add_and_double = add_and_double1 : reordered to match implementation **)
-op add_and_double1 (qx : zp) (nqs : (zp * zp) * (zp * zp)) =
+op op_add_and_double (qx : zp, nqs : (zp * zp) * (zp * zp)) : (zp * zp) * (zp * zp)  =
   let x1 = qx in
   let (x2, z2) = nqs.`1 in
   let (x3, z3) = nqs.`2 in
@@ -65,115 +52,118 @@ op add_and_double1 (qx : zp) (nqs : (zp * zp) * (zp * zp)) =
   let z2 = t0 * t2
   in  ((x2,z2), (x3,z3)).
 
-lemma eq_add_and_double1 (qx : zp) (nqs : (zp * zp) * (zp * zp)) :
-  add_and_double qx nqs = add_and_double1 qx nqs.
+(* lemma: spec_add_and_double = op_add_and_double *)
+lemma eq_op_add_and_double (qx : zp, nqs : (zp * zp) * (zp * zp)) :
+  spec_add_and_double qx nqs = op_add_and_double qx nqs.
 proof.
-  rewrite /add_and_double /add_and_double1.
-  simplify => /#.
+  rewrite /spec_add_and_double /op_add_and_double.
+  auto => />. smt().
 qed.
 
-op montgomery_ladder1(init : zp, k : W256.t) =
+(** step 2: montgomery ladder and isolate foldl function and introduce reconstruct tuple **)
+op op_montgomery_ladder1 (init : zp, k : W256.t) : (zp * zp) * (zp * zp) =
   let nqs0 = ((Zp.one,Zp.zero),(init,Zp.one)) in
   foldl (fun (nqs : (zp * zp) * (zp * zp)) ctr =>
-         if ith_bit k ctr
-         then swap_tuple (add_and_double1 init (swap_tuple(nqs)))
-         else add_and_double1 init nqs) nqs0 (rev (iota_ 0 255)).
+         if spec_ith_bit k ctr
+         then spec_swap_tuple (op_add_and_double init (spec_swap_tuple(nqs)))
+         else op_add_and_double init nqs) nqs0 (rev (iota_ 0 255)).
 
-(* lemma: montgomery_ladder = montgomery_ladder1 *)
-lemma eq_montgomery_ladder1 (init : zp) (k : W256.t) :
-  montgomery_ladder init k = montgomery_ladder1 init k.
-proof.
-  rewrite /montgomery_ladder /montgomery_ladder1 /=.
+
+op op_montgomery_ladder2_step(k : W256.t, init : zp, nqs : (zp * zp) * (zp * zp), ctr : int) : (zp * zp) * (zp * zp)=
+  if spec_ith_bit k ctr
+  then spec_swap_tuple(op_add_and_double init (spec_swap_tuple(nqs)))
+  else op_add_and_double init nqs.
+
+op op_montgomery_ladder2(init : zp, k : W256.t) : (zp * zp) * (zp * zp) =
+  let nqs0 = reconstruct_triple ((Zp.one,Zp.zero),(init,Zp.one),false) in
+  foldl (op_montgomery_ladder2_step k init) nqs0 (rev (iota_ 0 255)).
+
+(* lemma: spec_montgomery_ladder = op_montgomery_ladder1 *)
+lemma eq_op_montgomery_ladder1 (init : zp) (k : W256.t) :
+  spec_montgomery_ladder init k = op_montgomery_ladder1 init k.
+ proof.
+  rewrite /spec_montgomery_ladder /op_montgomery_ladder1 /=.
   apply foldl_in_eq.
   move => nqs ctr inlist => /=.
-  case (ith_bit k ctr).
-    by move => ?; rewrite /swap_tuple /#.
-    by move => ?; rewrite /swap_tuple /#.
-qed.
+  case (spec_ith_bit k ctr).
+      by move => ?; rewrite /spec_swap_tuple /#.
+  by move => ?; rewrite /spec_swap_tuple /#.
+ qed.
 
-(** step 2: isolate foldl function and introduce reconstruct tuple **)
-op montgomery_ladder2_step(k : W256.t, init : zp, nqs : (zp * zp) * (zp * zp), ctr : int) =
-  if ith_bit k ctr
-  then swap_tuple(add_and_double1 init (swap_tuple(nqs)))
-  else add_and_double1 init nqs.
-
-op montgomery_ladder2(init : zp, k : W256.t) =
-  let nqs0 = reconstruct_tuple ((Zp.one,Zp.zero),(init,Zp.one),false) in
-  foldl (montgomery_ladder2_step k init) nqs0 (rev (iota_ 0 255)).
-
-(* lemma: montgomery_ladder1 = montgomery_ladder2 *)
-lemma eq_montgomery_ladder2 (init : zp) (k : W256.t) :
-  montgomery_ladder1 init k = montgomery_ladder2 init k.
+(* lemma: op_montgomery_ladder1 = op_montgomery_ladder2 *)
+lemma eq_op_montgomery_ladder2 (init : zp) (k : W256.t) :
+  op_montgomery_ladder1 init k = op_montgomery_ladder2 init k.
 proof.
-  rewrite /montgomery_ladder1 /montgomery_ladder2 /reconstruct_tuple /select_tuple_12.
-  rewrite /montgomery_ladder2_step.
+  rewrite /op_montgomery_ladder1 /op_montgomery_ladder2 /reconstruct_triple /select_double_from_triple.
+  rewrite /op_montgomery_ladder2_step.
   by simplify.
 qed.
 
-(** step 3: extend the state to contain an additional bit stating if the state is swapped **)
-op cswap( t : ('a * 'a) * ('a * 'a), b : bool ) =
+
+(** step 3: extend the state to contain an additional bit stating if the state is swapped * *)
+
+op cswap (t : ('a * 'a) * ('a * 'a), b : bool) : ('a * 'a) * ('a * 'a)  =
   if b
-  then swap_tuple t
+  then spec_swap_tuple t
   else t.
 
-op montgomery_ladder3_step(k : W256.t, init : zp, nqs : (zp * zp) * (zp * zp) * bool, ctr : int) =
-  let nqs = cswap (select_tuple_12 nqs) (nqs.`3 ^^ (ith_bit k ctr)) in
-  let nqs = add_and_double1 init nqs in
-  (nqs.`1, nqs.`2, (ith_bit k ctr)).
+op op_montgomery_ladder3_step(k : W256.t, init : zp, nqs : (zp * zp) * (zp * zp) * bool, ctr : int) : (zp * zp) * (zp * zp) * bool =
+  let nqs = cswap (select_double_from_triple nqs) (nqs.`3 ^^ (spec_ith_bit k ctr)) in
+  let nqs = op_add_and_double init nqs in
+  (nqs.`1, nqs.`2, (spec_ith_bit k ctr)).
 
-op montgomery_ladder3(init : zp, k : W256.t) =
-  let nqs0 = ((Zp.one,Zp.zero),(init,Zp.one),false) in
-  foldl (montgomery_ladder3_step k init) nqs0 (rev (iota_ 0 255)).
+op op_montgomery_ladder3(init : zp, k : W256.t) : (zp * zp) * (zp * zp) * bool =
+  let nqs0 = ((Zp.one, Zp.zero),(init, Zp.one),false) in
+  foldl (op_montgomery_ladder3_step k init) nqs0 (rev (iota_ 0 255)).
 
-lemma eq_montgomery_ladder3_reconstruct (init : zp) (k: W256.t) :
-  montgomery_ladder2 init k = reconstruct_tuple (montgomery_ladder3 init k).
+(** lemma: op_montgomery_ladder2 = op_reconstruct_triple(op_montgomery_ladder3 ) **)
+lemma eq_op_montgomery_ladder3_reconstruct (init : zp) (k: W256.t) :
+  op_montgomery_ladder2 init k = reconstruct_triple (op_montgomery_ladder3 init k).
 proof.
-  rewrite /montgomery_ladder2 /montgomery_ladder3 //=.
+  rewrite /op_montgomery_ladder2 /op_montgomery_ladder3 //=.
   apply foldl_in_eq_r.
   move => ? ? ?.
-  rewrite /reconstruct_tuple /montgomery_ladder2_step /montgomery_ladder3_step.
-  rewrite /swap_tuple /select_tuple_12 /cswap.
+  rewrite /reconstruct_triple /op_montgomery_ladder2_step /op_montgomery_ladder3_step.
+  rewrite /spec_swap_tuple /select_double_from_triple /cswap.
   simplify => /#.
 qed.
 
-(* lemma: if the first bit of k is 0, which will be because of decodeScalar25519, *)
-(*  then montgomery_ladder2 = select_tuple_12 montgomery_ladder3 *)
-lemma eq_montgomery_ladder3 (init : zp) (k: W256.t) :
+(* lemma: if the first bit of k is 0, which will be because of spec_decode_scalar_25519, *)
+(*  then op_montgomery_ladder2 = select_double_from_triple op_montgomery_ladder3 *)
+lemma eq_op_montgomery_ladder3 (init : zp, k: W256.t) :
   k.[0] = false =>
-  montgomery_ladder2 init k = select_tuple_12 (montgomery_ladder3 init k).
+  op_montgomery_ladder2 init k = select_double_from_triple (op_montgomery_ladder3 init k).
 proof.
   move => hkf.
-  have tbf : (montgomery_ladder3 init k).`3 = false. (*third bit false*)
-    rewrite /montgomery_ladder3 /montgomery_ladder3_step /select_tuple_12 /cswap /ith_bit.
-    by simplify rev.
-  have seqr : select_tuple_12 (montgomery_ladder3 init k) = (*select eq reconstruct*)
-              reconstruct_tuple (montgomery_ladder3 init k).
-    by apply /eq_reconstruct_select_tuple /tbf.
+  have tbf : (op_montgomery_ladder3 init k).`3 = false. (*third bit false *)
+    rewrite /op_montgomery_ladder3 /op_montgomery_ladder3_step /select_double_from_triple /cswap /spec_ith_bit /spec_swap_tuple => />.
+    rewrite foldl_rev; auto => />; rewrite -iotaredE => />.
+  have seqr : select_double_from_triple (op_montgomery_ladder3 init k) = reconstruct_triple (op_montgomery_ladder3 init k).
+    by apply /eq_reconstruct_select_triple /tbf.
   rewrite seqr.
-    by apply eq_montgomery_ladder3_reconstruct.
+    by apply eq_op_montgomery_ladder3_reconstruct.
 qed.
 
-(** step 4: montgomery_ladder = select_tuple_12 montgomery_ladder3 **)
-lemma eq_montgomery_ladder123 (init : zp) (k: W256.t) :
-  k.[0] = false =>
-  montgomery_ladder init k = select_tuple_12 (montgomery_ladder3 init k).
+(** step 4: spec_montgomery_ladder = select_double_from_triple op_montgomery_ladder3 * *)
+lemma eq_op_montgomery_ladder123 (init : zp, k: W256.t) :
+  k.[0] = false => spec_montgomery_ladder init k = select_double_from_triple (op_montgomery_ladder3 init k).
 proof.
-  move => hkf.
-  by rewrite eq_montgomery_ladder1 eq_montgomery_ladder2 eq_montgomery_ladder3.
+  move => H.
+   rewrite eq_op_montgomery_ladder1 eq_op_montgomery_ladder2 eq_op_montgomery_ladder3. apply H. trivial.
 qed.
 
 (** step 5: introduce reordering in encode point **)
 (*  - we split invert in 3 parts to make the proof faster *)
-op invert_p_p1(z1 : zp) : (zp*zp) =
-  let z2 = exp z1 2 in
-  let z8 = exp z2 (2*2) in
+op op_invert_p_p1 (z1 : zp) : (zp * zp) =
+  let z2 = ZModpRing.exp z1 2 in
+  let z8 = ZModpRing.exp z2 (2*2) in
   let z9 = z1 * z8 in
   let z11 = z2 * z9 in
-  let z22 = exp z11 2 in
+  let z22 = ZModpRing.exp z11 2 in
   let z_5_0 = z9 * z22 in
   (z_5_0, z11).
 
-op invert_p_p2(z_5_0 : zp) : zp =
+op op_invert_p_p2(z_5_0 : zp) : zp =
   let z_10_5 = ZModpRing.exp z_5_0 (2^5) in
   let z_10_0 = z_10_5 * z_5_0 in
   let z_20_10 = ZModpRing.exp z_10_0 (2^10) in
@@ -184,7 +174,7 @@ op invert_p_p2(z_5_0 : zp) : zp =
   let z_50_0 = z_50_10 * z_10_0 in
   z_50_0.
 
-op invert_p_p3(z_50_0 z11 : zp) : zp =
+op op_invert_p_p3(z_50_0 z11 : zp) : zp =
   let z_100_50 = ZModpRing.exp z_50_0 (2^50) in
   let z_100_0 = z_100_50 * z_50_0 in
   let z_200_100 = ZModpRing.exp z_100_0 (2^100) in
@@ -195,40 +185,44 @@ op invert_p_p3(z_50_0 z11 : zp) : zp =
   let z_255_21 = z_255_5 * z11 in
   z_255_21.
 
-op invert_p(z1 : zp) : zp =
-  let (z_5_0, z11) = invert_p_p1 z1 in
-  let z_50_0 = invert_p_p2 z_5_0 in
-  let z_255_21 = invert_p_p3 z_50_0 z11 in
-  z_255_21 axiomatized by invert_pE.
+op op_invert_p(z1 : zp) : zp =
+  let (z_5_0, z11) = op_invert_p_p1 z1 in
+  let z_50_0 = op_invert_p_p2 z_5_0 in
+  let z_255_21 = op_invert_p_p3 z_50_0 z11 in
+  z_255_21 axiomatized by op_invert_pE.
 
-lemma eq_invert_p (z1: zp) :
-  invert_p z1 = ZModpRing.exp z1 (p-2).
+(* lemma: invert is the same as z1^(p-2) from fermat's little theorem *)
+
+lemma eq_op_invert_p (z1: zp) :
+  op_invert_p z1 = ZModpRing.exp z1 (p-2).
 proof.
-rewrite invert_pE.
-(*invert_p1*)
-rewrite /invert_p_p1 /= expE //=.
-  cut -> : invert_p_p3 (invert_p_p2 (z1 * exp z1 8 *
-                exp (exp z1 2 * (z1 * exp z1 8)) 2))
-                    (exp z1 2 * (z1 * exp z1 8)) =
-           invert_p_p3 (invert_p_p2 (exp z1 (2^5 - 2^0))) (exp z1 11).
-           smt(expE exprS exprD).
-(*invert_p2*)
-rewrite /invert_p_p2 //=.
-  cut -> : invert_p_p3 (exp (exp (exp
-                     (exp (exp z1 31) 32 * exp z1 31) 1024 *
-                     (exp (exp z1 31) 32 * exp z1 31)) 1048576 *
-                (exp (exp (exp z1 31) 32 * exp z1 31) 1024 *
-                     (exp (exp z1 31) 32 * exp z1 31))) 1024 *
-                     (exp (exp z1 31) 32 * exp z1 31)) (exp z1 11) =
-           invert_p_p3 (exp z1 (2^50 - 2^0)) (exp z1 11).
-           smt(expE exprS exprD).
-(*invert_p3*)
-rewrite /invert_p_p3 //= pE //=.
-smt(expE exprS exprD).
+    rewrite op_invert_pE.
+    rewrite /op_invert_p_p1 /= expE //= /op_invert_p_p3 /op_invert_p_p2 => />.
+    rewrite -!ZModpRing.exprS => />.
+    rewrite -!ZModpRing.exprD_nneg => />.
+    rewrite -!ZModpRing.exprM => />.
+    rewrite -!ZModpRing.exprD_nneg => />.
+    rewrite -!ZModpRing.exprM => />.
+    rewrite -!ZModpRing.exprD_nneg => />.
+    rewrite -!ZModpRing.exprM => />.
+    rewrite -!ZModpRing.exprD_nneg => />.
+    rewrite -!ZModpRing.exprM => />.
+    rewrite -!ZModpRing.exprD_nneg => />.
+    rewrite -!ZModpRing.exprM => />.
+    rewrite -!ZModpRing.exprD_nneg => />.
+    rewrite -!ZModpRing.exprM => />.
+    rewrite -!ZModpRing.exprD_nneg => />.
+    rewrite -!ZModpRing.exprM => />.
+    rewrite -!ZModpRing.exprD_nneg => />.
+    rewrite -!ZModpRing.exprM => />.
+    rewrite -ZModpRing.exprD_nneg => />.
+    rewrite -ZModpRing.exprM => />.
+    rewrite -!ZModpRing.exprD_nneg => />.
+    rewrite pE => />.
 qed.
 
 (* now we define invert as one op and prove it equiv to exp z1 (p-2) *)
-op invert0(z1 : zp) : zp =
+op op_invert0(z1 : zp) : zp =
   let z2 = ZModpRing.exp z1 2 in
   let z8 = ZModpRing.exp z2 (2*2) in
   let z9 = z1 * z8 in
@@ -251,152 +245,314 @@ op invert0(z1 : zp) : zp =
   let z_250_0 = z_250_50 * z_50_0 in
   let z_255_5 = ZModpRing.exp z_250_0 (2^5) in
   let z_255_21 = z_255_5 * z11 in
-  z_255_21 axiomatized by invert0E.
+  z_255_21 axiomatized by op_invert0E.
 
-lemma eq_invert0 (z1 : zp) :
-  invert0 z1 = invert_p z1.
+(* lemma: op_invert0 = op_invert_p *)
+lemma eq_op_invert0 (z1 : zp) :
+  op_invert0 z1 = op_invert_p z1.
 proof.
-  rewrite invert0E invert_pE /invert_p_p1 /invert_p_p2 /invert_p_p3 //.
+  rewrite op_invert0E op_invert_pE /op_invert_p_p1 /op_invert_p_p2 /op_invert_p_p3 //.
 qed.
 
-lemma eq_invert0p (z1 : zp) :
-  invert0 z1 = ZModpRing.exp z1 (p-2).
+(* lemma: hence, op_invert0 is equal to z1^(p-1) *)
+lemma eq_op_invert0p (z1 : zp) :
+  op_invert0 z1 = ZModpRing.exp z1 (p-2).
 proof.
-  rewrite eq_invert0 eq_invert_p //.
+  rewrite eq_op_invert0 eq_op_invert_p //.
 qed.
 
-op sqr(z : zp) : zp =
+(* we now need to define various iterated sqaure operations and lemmas *)
+op op_sqr(z : zp) : zp =
  ZModpRing.exp z 2.
 
-op it_sqr(e : int, z : zp) : zp =
+op op_it_sqr(e : int, z : zp) : zp =
   ZModpRing.exp z (2^e).
 
-op it_sqr1(e : int, z : zp) : zp =
-  foldl (fun (z' : zp) _ => exp z' 2) z (iota_ 0 e).
+op op_it_sqr1(e : int, z : zp) : zp =
+  foldl (fun (z' : zp) _ => ZModpRing.exp z' 2) z (iota_ 0 e).
 
-lemma eq_it_sqr1 (e : int, z : zp) :
+op op_it_sqr_x2(e : int, z : zp) : zp =
+    ZModpRing.exp z (4^e).
+
+op op_it_sqr1_x2(e : int, z : zp) : zp =
+    foldl (fun (z' : zp) _ => ZModpRing.exp z' 4) z (iota_ 0 e).
+
+(* lemma: op_it_sqr1 = op_itr_sqr *)
+lemma eq_op_it_sqr1 (e : int, z : zp) :
   0 <= e  =>
-  it_sqr1 e z = it_sqr e z.
+  op_it_sqr1 e z = op_it_sqr e z.
 proof.
   move : e.
-  rewrite /it_sqr1 /it_sqr. elim. by simplify; smt(expr1).
+  rewrite /op_it_sqr1 /op_it_sqr. elim. simplify. rewrite -iotaredE ZModpRing.expr1 //.
   move => i ige0 hin.
-  rewrite iotaSr // -cats1 foldl_cat hin /= expE /=. smt(gt0_pow2).
+  rewrite iotaSr // -cats1 foldl_cat hin /= expE /=.  smt(gt0_pow2).
   congr. clear hin.
-  rewrite powS // mulzC //.
+  rewrite exprS // mulzC //.
 qed.
 
-op invert1(z1 : zp) : zp =
-  let t0 = sqr z1  in        (* z1^2  *)
-  let t1 = sqr t0  in        (* z1^4  *)
-  let t1 = sqr t1  in        (* z1^8  *)
+(* lemma: op_it_sqr1_x2 = op_itr_sqr_x2 *)
+lemma eq_op_it_sqr1_x2 (e : int, z : zp) :
+  0 <= e  =>
+  op_it_sqr1_x2 e z = op_it_sqr_x2 e z.
+proof.
+  move : e.
+  rewrite /op_it_sqr1_x2 /op_it_sqr_x2. elim. simplify. rewrite -iotaredE ZModpRing.expr1 //.
+  move => i ige0 hin.
+  rewrite iotaSr // -cats1 foldl_cat hin /= expE /=.
+  have ->: 4^i = 2^2^i. rewrite expr2 //.
+  rewrite -exprM. smt(gt0_pow2).
+  congr. clear hin.
+  rewrite exprS // mulzC //.
+qed.
+
+(* lemma: op_it_sqr = op_itr_sqr_x2 *)
+lemma eq_op_it_sqr_x2_4 (e : int, z : zp) :
+  0 <= e  => e %% 2 = 0 =>
+  op_it_sqr e z = op_it_sqr_x2 (e%/2) z.
+proof.
+  move => e1 e2.
+  rewrite /op_it_sqr /op_it_sqr_x2.
+  congr.
+  have ->: 4 ^ (e %/ 2) = 2 ^ 2 ^ (e %/ 2). rewrite expr2 => />.
+  rewrite -exprM => />. smt().
+qed.
+
+(* lemma: op_it_sqr1 = op_itr1_sqr_x2 *)
+lemma eq_op_it_sqr1_x2_4 (e : int, z : zp) :
+  0 <= e  => e %% 2 = 0 =>
+  op_it_sqr1 e z = op_it_sqr1_x2 (e%/2) z.
+proof.
+  move => H H0.
+  rewrite eq_op_it_sqr1 // eq_op_it_sqr1_x2. smt().
+  apply eq_op_it_sqr_x2_4; trivial.
+qed.
+
+(* lemma: op_it_sqr1 = op_itr_sqr_x2, other perspective *)
+lemma eq_op_it_sqr1_x2_4_twice (e : int, z : zp) :
+  0 <= e  => e %% 2 = 0 =>
+  op_it_sqr1 (2*e) z = op_it_sqr1_x2 e z.
+proof.
+  move => H H0.
+  rewrite eq_op_it_sqr1 //. smt(). rewrite eq_op_it_sqr1_x2. smt().
+  rewrite /op_it_sqr /op_it_sqr_x2 => />.
+  have ->: 4 ^ e = 2 ^ 2 ^ e. rewrite expr2 => />.
+  rewrite -exprM => />.
+qed.
+
+(* lemma: op_it_sqr1 with arg 0 *)
+lemma op_it_sqr1_0 (e : int) (z : zp) :
+   0 = e => op_it_sqr1 e z = z.
+proof.
+  move => ?.
+  rewrite eq_op_it_sqr1. smt().
+  rewrite /op_it_sqr. subst. simplify.
+  rewrite ZModpRing.expr1 //.
+qed.
+
+(* lemma: op_it_sqr1_x2 with arg 0 *)
+lemma op_it_sqr1_x2_0 (e : int) (z : zp) :
+  0 = e => op_it_sqr1_x2 e z = z.
+proof.
+  move => ?.
+  rewrite eq_op_it_sqr1_x2. smt().
+  rewrite /op_it_sqr_x2. subst. simplify.
+  rewrite ZModpRing.expr1 //.
+qed.
+
+(* lemma: "decomposing" op_it_sqr1 with e-2 *)
+lemma op_it_sqr1_m2_exp4 (e : int) (z : zp) :
+   0 <= e - 2 => op_it_sqr1 e z = op_it_sqr1 (e-2) (ZModpRing.exp (ZModpRing.exp z 2) 2).
+proof.
+  rewrite expE // /= => ?.
+  rewrite !eq_op_it_sqr1. smt(). trivial.
+  rewrite /op_it_sqr (*expE *).
+  (* directly rewriting expE takes too long *)
+  have ee :  ZModpRing.exp (ZModpRing.exp z 4) (2 ^ (e - 2)) =  ZModpRing.exp z (2^2 * 2 ^ (e - 2)). smt(expE).
+  rewrite ee. congr.
+  rewrite -exprD_nneg //.
+qed.
+
+(* lemma: "decomposing" op_it_sqr1 witg arg e-1 *)
+lemma op_it_sqr1_m2_exp1 (e : int) (z : zp) :
+   0 <= e - 1 => op_it_sqr1 e z = op_it_sqr1 (e-1) (ZModpRing.exp z  2).
+proof.
+  have ->: ZModpRing.exp z 2 = ZModpRing.exp (ZModpRing.exp z 1) 2. rewrite expE. smt(). trivial.
+  rewrite expE // /= => ?.
+  rewrite !eq_op_it_sqr1. smt(). smt().
+  rewrite /op_it_sqr (*expE *). rewrite expE. split. smt().
+  rewrite expr_ge0 //. congr. have ->: 2 * 2^(e-1) = 2^1 * 2^(e-1). rewrite expr1 //.
+  rewrite -exprD_nneg //.
+qed.
+
+(* lemma: "decomposing" op_it_sqr1_x2 with arg e-2 *)
+lemma op_it_sqr1_m2_exp4_x2 (e : int) (z : zp) :
+   0 <= e - 2 => op_it_sqr1_x2 e z = op_it_sqr1_x2 (e-2) (ZModpRing.exp (ZModpRing.exp z 4) 4).
+proof.
+  have E: 4^(e-2) = 2^(2*(e-2)) by rewrite exprM => />.
+  rewrite expE // /= => H.
+  rewrite !eq_op_it_sqr1_x2. smt(). trivial.
+  rewrite /op_it_sqr_x2.
+  rewrite expE. rewrite E. smt(gt0_pow2).
+  congr => />.  have ->: 16 = 4^2 by rewrite expr2.
+  rewrite -exprD_nneg //.
+qed.
+
+(* lemma: "decomposing" op_it_sqr1_x2 with arg e-1 *)
+lemma op_it_sqr1_m2_exp1_x2 (e : int) (z : zp) :
+  0 <= e - 1 => op_it_sqr1_x2 e z = op_it_sqr1_x2 (e-1) (ZModpRing.exp z 4).
+proof.
+  have ->: ZModpRing.exp z 4 = ZModpRing.exp (ZModpRing.exp z 1) 4. rewrite expE. smt(). trivial.
+  rewrite expE // /= => ?.
+  rewrite !eq_op_it_sqr1_x2. smt(). smt().
+  rewrite /op_it_sqr_x2 (*expE *). rewrite expE. split. smt().
+  rewrite expr_ge0 //. congr. have ->: 4 * 4^(e-1) = 4^1 * 4^(e-1). rewrite expr1 //.
+  rewrite -exprD_nneg //.
+qed.
+
+op op_invert1(z1 : zp) : zp =
+  let t0 = op_sqr z1  in        (* z1^2  *)
+  let t1 = op_sqr t0  in        (* z1^4  *)
+  let t1 = op_sqr t1  in        (* z1^8  *)
   let t1 = z1 * t1 in        (* z1^9  *)
   let t0 = t0 * t1 in        (* z1^11 *)
-  let t2 = sqr t0  in        (* z1^22 *)
+  let t2 = op_sqr t0  in        (* z1^22 *)
   let t1 = t1 * t2 in        (* z_5_0  *)
-  let t2 = sqr t1  in        (* z_10_5 *)
-  let t2 = it_sqr 4 t2  in
+  let t2 = op_sqr t1  in        (* z_10_5 *)
+  let t2 = op_it_sqr 4 t2  in
   let t1 = t1 * t2 in        (* z_10_0 *)
-  let t2 = it_sqr 10 t1 in   (* z_20_10 *)
+  let t2 = op_it_sqr 10 t1 in   (* z_20_10 *)
   let t2 = t1 * t2 in        (* z_20_0 *)
-  let t3 = it_sqr 20 t2 in   (* z_40_20 *)
+  let t3 = op_it_sqr 20 t2 in   (* z_40_20 *)
   let t2 = t2 * t3 in        (* z_40_0 *)
-  let t2 = it_sqr 10 t2 in   (* z_50_10 *)
+  let t2 = op_it_sqr 10 t2 in   (* z_50_10 *)
   let t1 = t1 * t2 in        (* z_50_0 *)
-  let t2 = it_sqr 50 t1 in   (* z_100_50 *)
+  let t2 = op_it_sqr 50 t1 in   (* z_100_50 *)
   let t2 = t1 * t2 in        (* z_100_0 *)
-  let t3 = it_sqr 100 t2 in  (* z_200_100 *)
+  let t3 = op_it_sqr 100 t2 in  (* z_200_100 *)
   let t2 = t2 * t3 in        (* z_200_0 *)
-  let t2 = it_sqr 50 t2 in   (* z_250_50 *)
+  let t2 = op_it_sqr 50 t2 in   (* z_250_50 *)
   let t1 = t1 * t2 in        (* z_250_0 *)
-  let t1 = it_sqr 4 t1 in    (* z_255_5 *)
-  let t1 = sqr t1 in
+  let t1 = op_it_sqr 4 t1 in    (* z_255_5 *)
+  let t1 = op_sqr t1 in
   let t1 = t0 * t1 in
-  t1 axiomatized by invert1E.
+  t1 axiomatized by op_invert1E.
 
-lemma eq_invert1 (z1: zp) :
-  invert1 z1 = invert0 z1.
+(* lemma: op_invert1 = op_invert0 *)
+lemma eq_op_invert1 (z1: zp) :
+  op_invert1 z1 = op_invert0 z1.
 proof.
- rewrite invert1E invert0E /= /it_sqr /sqr /=.
+ rewrite op_invert1E op_invert0E /= /op_it_sqr /op_sqr /=.
  smt(exprS exprD expE).
 qed.
 
 (** split invert2 in 3 parts : jump from it_sqr to it_sqr1 **)
 
-op invert2(z1 : zp) : zp =
-  let t0 = sqr z1  in        (* z1^2  *)
-  let t1 = sqr t0  in        (* z1^4  *)
-  let t1 = sqr t1  in        (* z1^8  *)
+op op_invert2(z1 : zp) : zp =
+  let t0 = op_sqr z1  in        (* z1^2  *)
+  let t1 = op_sqr t0  in        (* z1^4  *)
+  let t1 = op_sqr t1  in        (* z1^8  *)
   let t1 = z1 * t1 in        (* z1^9  *)
   let t0 = t0 * t1 in        (* z1^11 *)
-  let t2 = sqr t0  in        (* z1^22 *)
+  let t2 = op_sqr t0  in        (* z1^22 *)
   let t1 = t1 * t2 in        (* z_5_0  *)
-  let t2 = sqr t1  in        (* z_10_5 *)
-  let t2 = it_sqr1 4 t2  in
+  let t2 = op_sqr t1  in        (* z_10_5 *)
+  let t2 = op_it_sqr1 4 t2  in
   let t1 = t1 * t2 in        (* z_10_0 *)
-  let t2 = it_sqr1 10 t1 in  (* z_20_10 *)
+  let t2 = op_it_sqr1 10 t1 in  (* z_20_10 *)
   let t2 = t1 * t2 in        (* z_20_0 *)
-  let t3 = it_sqr1 20 t2 in  (* z_40_20 *)
+  let t3 = op_it_sqr1 20 t2 in  (* z_40_20 *)
   let t2 = t2 * t3 in        (* z_40_0 *)
-  let t2 = it_sqr1 10 t2 in  (* z_50_10 *)
+  let t2 = op_it_sqr1 10 t2 in  (* z_50_10 *)
   let t1 = t1 * t2 in        (* z_50_0 *)
-  let t2 = it_sqr1 50 t1 in  (* z_100_50 *)
+  let t2 = op_it_sqr1 50 t1 in  (* z_100_50 *)
   let t2 = t1 * t2 in        (* z_100_0 *)
-  let t3 = it_sqr1 100 t2 in (* z_200_100 *)
+  let t3 = op_it_sqr1 100 t2 in (* z_200_100 *)
   let t2 = t2 * t3 in        (* z_200_0 *)
-  let t2 = it_sqr1 50 t2 in  (* z_250_50 *)
+  let t2 = op_it_sqr1 50 t2 in  (* z_250_50 *)
   let t1 = t1 * t2 in        (* z_250_0 *)
-  let t1 = it_sqr1 4 t1 in   (* z_255_5 *)
-  let t1 = sqr t1 in
+  let t1 = op_it_sqr1 4 t1 in   (* z_255_5 *)
+  let t1 = op_sqr t1 in
   let t1 = t0 * t1 in
-  t1 axiomatized by invert2E.
+  t1 axiomatized by op_invert2E.
 
-lemma eq_invert2 (z1: zp) :
-  invert2 z1 = invert1 z1.
+
+(* lemma: op_invert2 = op_invert 1 *)
+lemma eq_op_invert2 (z1: zp) :
+  op_invert2 z1 = op_invert1 z1.
 proof.
-  rewrite invert2E invert1E. smt(eq_it_sqr1).
+  rewrite op_invert2E op_invert1E. smt(eq_op_it_sqr1).
 qed.
 
-lemma eq_invert210p (z1: zp) :
-  invert2 z1 = ZModpRing.exp z1 (p-2).
+(* lemma: op_invert2 returns the inverse of its arg *)
+lemma eq_op_invert210p (z1: zp) :
+  op_invert2 z1 = ZModpRing.exp z1 (p-2).
 proof.
-rewrite eq_invert2 eq_invert1 eq_invert0p //.
+  rewrite eq_op_invert2 eq_op_invert1 eq_op_invert0p //.
 qed.
 
-(* now we define an alternative version of encodePoint *)
-op encodePoint1 (q: zp * zp) : W256.t =
-  let qi = invert2 q.`2 in
-  let q = q.`1 * qi in
-      W256.of_int (asint q) axiomatized by encodePoint1E.
+(* now we define an alternative version of spec_encode_point *)
+op op_encode_point (q: zp * zp) : W256.t =
+  let qi = op_invert2 q.`2 in
+  let q =  q.`1 * qi in
+      W256.of_int (asint q) axiomatized by op_encode_pointE.
 
-lemma eq_encodePoint1 (q: zp * zp) :
-  encodePoint1 q = encodePoint q.
+(* lemma: op_encode_point = spec_encode_point *)
+lemma eq_op_encode_point (q: zp * zp) :
+  op_encode_point q = spec_encode_point q.
 proof.
-  rewrite encodePoint1E encodePointE. simplify. congr.
-  rewrite eq_invert210p //.
+  rewrite op_encode_pointE spec_encode_pointE. simplify. congr.
+  rewrite eq_op_invert210p //.
 qed.
 
-(** step 6: scalarmult with updated montgomery_ladder3 **)
-op scalarmult1 (k:W256.t) (u:W256.t) : W256.t =
-  let k = decodeScalar25519 k in
-  let u = decodeUCoordinate u in
-  let r = montgomery_ladder3 u k in
-      encodePoint1 (r.`1) axiomatized by scalarmult1E.
+(* step 6: spec_scalarmult with updated op_montgomery_ladder3 *)
 
-hint simplify scalarmult1E.
+op op_scalarmult_internal(u: zp, k:W256.t) : W256.t =
+  let r = op_montgomery_ladder3 u  k in
+    op_encode_point (r.`1) axiomatized by op_scalarmult_internalE.
 
-(* lemma scalarmult = scalarmult1 *)
-lemma eq_scalarmult1 (k:W256.t) (u:W256.t) :
-  scalarmult1 k u = scalarmult k u.
+(* lemma: spec_scalarmult = op_scalarmult *)
+lemma eq_op_scalarmult_internal (u:zp) (k:W256.t) :
+k.[0] = false => op_scalarmult_internal u k = spec_scalarmult_internal u k.
+proof.
+  rewrite /op_scalarmult_internal. simplify.
+  rewrite eq_op_encode_point /spec_scalarmult_internal. simplify. move => H.
+  congr.
+  have ml123 : spec_montgomery_ladder u k = select_double_from_triple (op_montgomery_ladder3 u k).
+  apply eq_op_montgomery_ladder123. apply H.
+  rewrite ml123 /select_double_from_triple //.
+qed.
+
+hint simplify op_scalarmult_internalE.
+
+op op_scalarmult (k:W256.t) (u:W256.t) : W256.t =
+  let k = spec_decode_scalar_25519 k in
+  let u = spec_decode_u_coordinate u in
+  op_scalarmult_internal (inzp (to_uint u)) k axiomatized by op_scalarmultE.
+
+hint simplify op_scalarmultE.
+
+op op_scalarmult_base(k:W256.t) : W256.t =
+  op_scalarmult (k) (W256.of_int(9%Int)).
+
+(* lemma: spec_scalarmult = op_scalarmult *)
+lemma eq_op_scalarmult (k:W256.t) (u:W256.t) :
+ op_scalarmult k u = spec_scalarmult k u.
 proof.
   simplify.
-  pose du := decodeUCoordinate u.
-  pose dk := decodeScalar25519 k.
-  rewrite eq_encodePoint1.
+  pose du := spec_decode_u_coordinate u.
+  pose dk := spec_decode_scalar_25519 k.
+  rewrite eq_op_encode_point /spec_scalarmult_internal. simplify.
   congr.
   have kb0f  : (dk).[0] = false. (* k bit 0 false *)
-    rewrite /dk /decodeScalar25519 //.
-  have ml123 : montgomery_ladder du dk = select_tuple_12 (montgomery_ladder3 du dk).
-    move : kb0f. apply eq_montgomery_ladder123.
-  rewrite ml123 /select_tuple_12 //.
+    rewrite /dk /spec_decode_scalar_25519 //.
+  have ml123 : spec_montgomery_ladder (inzp (to_uint du)) dk = select_double_from_triple (op_montgomery_ladder3 (inzp (to_uint du)) dk).
+    move : kb0f. apply eq_op_montgomery_ladder123.
+  rewrite ml123 /select_double_from_triple //.
+qed.
+
+(* lemma: spec_ op_scalarmult_base = spec_scalarmult_base *)
+lemma eq_op_scalarmult_base (k:W256.t) :
+  op_scalarmult_base k = spec_scalarmult_base k.
+proof.
+  apply eq_op_scalarmult.
 qed.
